## Sample Question

**L = { $a^{n}b^{n}c^{n} | n \geq 0$ }**

- S --> aSBc | $\epsilon$
    - In above we haven't written aSbc as then b and c will mix up.
    - This will create string like aaaBcBcBc
- Now, try to bring all BBB in between aaa and ccc
- cB --> Bc
   - This will swap and make string aaaBBBccc
- Fill only those b's which we can confirm they are with a's
- Look we can't write B --> b, as it will again create mix if used before cB --> Bc and in Grammar there are no rules like use one production rule after other, we can use anyone at anytime.
- So, to ensure B with a and change
- aB --> ab
- Again change all connected B with b
- bB --> bb
- Now, we have string aaabbbccc
- $\therefore$ Grammar:
    - S --> aSBc | $\epsilon$
    - cB --> Bc
    - aB --> ab
    - bB --> bb

**L = { $a^{n}b^{n}c^{n}d^{n} | n \geq 0$ }**
- S --> aSBCd | $\epsilon$
- dB --> Bd
- CB --> BC
- dC --> Cd
- aB --> ab
- bB --> bb
- bC --> bc
- cC --> cc
