### ⭐⭐⭐
- $b^{*}.(b^{*}.a.b^{*}.a.b^{*})^{*} + b^{*}.a.b^{*}(b^{*}.a.b^{*}.a.b^{*})^{*}$  
- = $(\epsilon + b^{*}.a).b^{*}.(b^{*}.a.b^{*}.a.b^{*})$ (Taking things common)  
- = $(a + b)^{*}$

### Important
- $(b^{*}.a.b^{*}) \Rightarrow$ R.E. for exact;y one a.
- $(b^{*}.a.b^{*})^{*} \Rightarrow$ R.E. for any number of a's.
- $(b^{*}.a.b^{*})^{+} \Rightarrow$ R.E. for atleast one a.

### ⭐⭐⭐ (GATE Favorite)
**Not aa as substring**
- For aa as substring we have R.E. = $(a + b)^{*}.aa.(a + b)^{*}$
- $(a + b)^{*} can generate any string over a & b.
- if we put constraint on it of it can't generate back-to-back 2 a's then R.E. = $(ab + b)^{*}$ but, it will not contain string like bab, aba, baba, etc.
- We can also see that the string will always end with b, we can't create end with a in it.
- Answer, $(ab + b)^{*}.(a + \epsilon)$
  - This can end either with a or b. Also it can generate only a.
- Another, $(a + \epsilon).(ba + b)^{*}$
- $\epsilon$ is added in above cases which gives flexibility to select with whcih letter we want to start or end.

**Strings containing aa or bb as substring**
- $(a + b)^{*}.aa.(a + b)^{*} + (a + b)^{*}.bb.(a + b)^{*}$  
  = $(a + b)^{*}.(aa + bb).(a + b)^{*}$

**Not aa as substring and not bb as substring**
- $(b + \epsilon).(ab)^{*}.(a + \epsilon)$ $\Leftrightarrow$ $(a + \epsilon).(ba)^{*}.(b + \epsilon)$

**R.E. to define variable in C**
- $l.(l + d)^{*}$

## Properties

1. R1 + R2 = R2 + R1
   - R1.R2 = R2.R1 ❌
2. R1 + (R2 + R3) = (R1 + R2) + R3
   - R1.(R2.R3) = (R1.R2).R3
3. R1.(R2 + R3) = R1.R2 + R1.R3
   - R1 + (R2.R3) = (R1 + R2).(R1 + R3) ❌
4. R1.$\epsilon$ = $\epsilon$.R1 = R1 (For 'Concatenation' $\epsilon$ is identity element)
5. R1 + $\phi$ = $\phi$ + R1 = R1 (For 'Union' $\phi$ is identity element)
6. R1 . $\phi$ = $\phi$ . R1 = $\phi$ (For 'Concatenation' $\phi$ is absorbing element)
7. R1 + R1 = R2 (If L(R1) $\subseteq$ L(R2))
   - $(a + b)^{*}.ba + (a + b)^{*}.a = (a + b)^{*}.a$