**Complement of atleast 1 a and atleast 1 b**
- 0 a's or 0 b's
- $a^{*} + b^{*}$

### Identity
- (a + b + anyString)* = (a + b)* 
- $((a + b)^{*})^{*} = (a + b)^{*}$
- $(a^{*} + b^{*})^{*} = (a + b)^{*}$
- $(a^{*}.b^{*})^{*} = (b^{*}.a^{*})^{*} = (a + b)^{*}$ ⭐⭐⭐⭐⭐(Gate Favourite)

**Even number of a's for string for a & b**
- We have exactly 2 a where b can be anywhere in between 
  - $b^{*}.a.b^{*}.a.b^{*}$
- For even number of a's, we can have 0 a's or 2 a's or 4 a's or 6 a's
  - $(b^{*}.a.b^{*}.a.b^{*})^{*} + b^{*}$
  - + b* is for 0 a's
- Another way,
  - $(b^{*}.a.b^{*}.a.b^{*})^{*}.b^{*}$

**Odd number of a's for string for a & b**
- We have even number of a's now if we add exactly 1 a, we will have odd number of a's
  - $(b^{*}.a.b^{*}.a.b^{*})^{*}.(b^{*}.a.b^{*})$


### ⭐⭐⭐
- **Can we have a regular expression where R1 + R2 = R1.R2?**  
Yes, as we have seen in the above example  
- **Can we have a regular expression where R1.R2 = R2.R1?**  
Yes  
- **$(R1^{*})^{+} = (R1^{+})^{*} = (R1^{*})^{*} = R1^{*}$**