### Create Grammar for the Language L = { $a^{m}b^{n} | m \le 2n$ }

- L = { $\epsilon$, b, bb, ab, aab, abb, aabb, aaabb, aaaabb}
- S -> aaSb | aSb | Sb | $\epsilon$
- At max we can have 2 a's for every b
- Apart from that either we can have 1 a for every b or no a for every b
- $\epsilon$ is the escape route

### Create Grammar for the Language L = { $a^{m}b^{n} | n \le 2m$ }

- S -> aS | aSbb | aSb | $\epsilon$

### Create Grammar for the Language L = { $a^{m}b^{n} | m \le 2n+3$ }

- First create for $m \le 2n$
- S -> aaSb | aSb | Sb | $\epsilon$
- Now at most we can add 3 b's to the right of the string
- $\therefore$ S -> aaSb | aSb | Sb | $\epsilon$ | A
- A -> a | aa | aaa

### Create Grammar for the Language L = { $a^{n}c^{m}b^{n}$ }

- S -> aSb | $\epsilon$ | cA
- A -> cA | $\epsilon$

### Create Grammar for the Language L = { $a^{n}c^{m}b^{n} | n,m \ge 1$ }

- Minimum string here will be acb
- S -> aSb | aAb
- A -> cA | c
- Generate any number of pairs of a and b through aSb
- Escape through aAb and genrate any number of Cs

### Create Grammar for the Language L = { $a^{n}c^{m}b^{n} | n \ge 0, m \ge 1$ }
- S -> aSb | cA
- A -> cA | $\epsilon$

### Create Grammar for the Language L = { $a^{n}c^{m}b^{n} | n \ge 1, m \ge 0$ }
- S -> aSb | aAb
- A -> cA | $\epsilon$

### Create Grammar for the Language L = { $a^{n}b^{n}c^{m} | n,m \ge 0$ }
- S -> S1A
- S1 -> aS1b | $\epsilon$
- A -> cA | $\epsilon$

### Create Grammar for the Language L = { $a^{n}b^{m}c^{m} | n,m \ge 0$ }
- S -> S1A
- S1 ->  aS1 | $\epsilon$
- A -> bAc | $\epsilon$

---
#### Create Grammar for the Language L = { $a^{n}b^{m}c^{m} | n,m \ge 1$ }
#### Create Grammar for the Language L = { $a^{n}b^{m}c^{m} | n \ge 1 m \ge 0$ }
#### Create Grammar for the Language L = { $a^{n}b^{m}c^{m} | n \ge 0 m \ge 1$ }
---

### Create Grammar for the Language L = { $a^{n}b^{m}c^{n+m} | n,m \ge 0$ }

- S -> aSc | A 
- A -> bAc | $\epsilon$

### Create Grammar for the Language L = { $a^{n+m}b^{m}c^{n} | n,m \ge 0$ }

- S -> A | aSc
- A -> aAb | $\epsilon$

### Create Grammar for the Language L = { $a^{n}b^{n+m}c^{m} | n,m \ge 0$ }

- S -> S1A
- S1 -> aS1b | $\epsilon$
- A -> bAc | $\epsilon$

### Create Grammar for the Language L = { $a^{n}b^{m}c^{n-m} | n,m \ge 0$ }

- First create pairs of ab and then escape and create pairs of ac
- S -> aSc | A
- A -> aAb | $\epsilon$

- Same as L = { $a^{n+m}b^{m}c^{n} | n,m \ge 0$ }
- To get the way check the power and try to make one equal to sum of other 2.
- Here m + (n-m) = n

### Create Grammar for the Language L = { $a^{n}b^{n}c^{m}d^{m} | n,m \ge 0$ }

- S -> S1S2
- S1 -> aS1b | $\epsilon$
- S2 -> cS2d | $\epsilon$

### Create Grammar for the Language L = { $a^{n}b^{m}c^{m}d^{n} | n,m \ge 0$ }

- S -> aSd | A
- A -> bAc | $\epsilon$

### Create Grammar for the Language L = { $a^{n}b^{m}c^{n}d^{m} | n,m \ge 0$ }
- Not a CFL ❌, it is a CSL✅

### Create Grammar for the Language L = { $(ab)^{n}(cd)^{m} | n,m \ge 0$ }

- L = {ababcdcd, abababcdcdcd, ababababcdcdcdcd, ...}
- S -> abS | cdS | $\epsilon$