## Construction of Regular Grammar

### For Construction Purpose we will use restricted definition of Regular Grammar
- RHS can be T/TN/$\epsilon$
- We can convert T*N to TN for example:
    - S -> aaS
    - then,
        - S -> aA
        - A -> aS
    - S -> aaaS
    - then,
        - S -> aA
        - A -> aB
        - B -> aS

### Construct a Regular Grammar which generate all Strings over a & b

- S -> aS | bS | $\epsilon$
- L = $\Sigma^*$ (Same as question)
- If option comes S -> aS | bS 
    - then L = $\phi$ as there won't be any termination
- If option comes S -> aS | bS | $\epsilon$ | a | b
    - then L = $\Sigma^*$ (adding a and b in RHS is useless)

- Even if with actual answer some other production rule is provided which does not generate any string then also it is correct
- Example:
    - S -> aS | bS | $\epsilon$ | bB
    - L = $\Sigma^*$
    - bB is useless

## Don't wander, hold the correct path (If unnecessary production rule is provided then also it is correct)

**>For any Regular Language we can have infinite Regular Grammar generating it**

### Construct a Regular Grammar which generate all Strings over a & b that ends with a

- S -> aS | bS | a

### Construct a Regular Grammar which generate all Strings over a & b that ends with aa

- S -> aS | bS | aA
- A -> a


### Construct a Regular Grammar which generate all Strings over a & b that starts with a

- S -> aA
- A -> aA | bA | $\epsilon$

### Construct a Regular Grammar which generate all Strings over a & b that starts with aa

- S -> aA
- A -> aB
- B -> aB | bB | $\epsilon$

### Construct a Regular Grammar which generate all Strings over a & b that starts and ends with a

- S -> aA | a
- A -> aA | bA | a

- if We would have written 
    - S -> aA
    - A -> aA | bA | a
    - then L will miss the smallest string which is a

### Construct a Regular Grammar which generate all Strings over a & b that starts with a and ends with b

- S -> aA
- A -> aA | bA | b 

### Construct a Regular Grammar which generate all Strings over a & b that starts and ends with different symbol

- S -> aA | bB
- A -> aA | bA | b
- B -> aB | bB | a

### Construct a Regular Grammar which generate all Strings over a & b that starts and ends with same symbol

- S -> aA | bB | a | b | $\epsilon$
- A -> aA | bA | a
- B -> aB | bB | b

### Question: S->aS|bS|a|b| 
- [x] A. All Possible strings over a and b that ends wih a or b
- [x] B. All Possible strings over a and b that starts with a or b
- [x] C. All Possible strings over a and b with length at least 1
- D. None

- A,B,C are correct
- L = {a,b,aa,ba,bb,aba,...}